formal/inference/Code_Target_Set.thy
@@ -1,0 +1,27 @@
+theory Code_Target_Set
+imports Main
+begin
+
+code_datatype set
+declare List.union_coset_filter [code del]
+declare insert_code [code del]
+declare remove_code [code del]
+declare card_coset_error [code del]
+declare coset_subseteq_set_code [code del]
+declare eq_set_code(1) [code del]
+declare eq_set_code(2) [code del]
+declare eq_set_code(4) [code del]
+declare List.subset_code [code del]
+declare inter_coset_fold [code del]
+declare subset_eq [code]
+
+(* Get rid of that one unnamed lemma *)
+lemma [code del]: "x \<in> List.coset xs \<longleftrightarrow> \<not> List.member xs x"
+  by (simp add: member_def)
+
+lemma sup_set_append [code]: "(set x) \<union> (set y) = set (x @ y)"
+  by simp
+
+declare product_concat_map [code]
+
+end
